proof/spec/DistrExtra.ec
@@ -1,0 +1,1225 @@
+require import AllCore List StdBigop StdOrder IntDiv Distr.
+(*---*) import IntOrder Bigint MUniform Range.
+
+
+(* ? Distr.ec *)
+
+import Bigreal Bigreal.BRA.
+
+lemma dlet1Efin ['a, 'b] (d : 'a distr) (f : 'a -> 'b distr) (b : 'b) s:
+  Finite.is_finite_for (support d) s =>
+  mu1 (dlet d f) b
+  = BRA.big predT (fun (a : 'a) => mu1 d a * mu1 (f a) b) s.
+proof.
+move=> [Hun H].
+rewrite dlet1E (RealSeries.sumE_fin _ s) //= => x.
+rewrite RField.unitrM; move=> [??].
+apply (H x); smt(ge0_mu1).
+qed.
+
+
+(* ? DBits.ec *)
+require import DInterval.
+
+abbrev dbits n = dinter 0 (2^n - 1).
+
+lemma dbits0: dbits 0 = dunit 0.
+proof.
+rewrite eq_distr => x.
+by rewrite dinter1E dunit1E expr0 /#.
+qed.
+
+lemma dprod_dbits k1 k2:
+  0 <= k1 => 0 <= k2 =>
+  dbits k1 `*` dbits k2
+  = dmap (dbits (k1+k2)) (fun x => (x%%2^k1, x%/2^k1)).
+proof.
+move=> Hk1 Hk2.
+rewrite eq_distr; move => [x1 x2].
+rewrite dprod1E dmap1E /(\o) !dinterE  /(=) /=.
+have L: forall x N, size (filter (pred1 x) (range 0 N)) = b2i (0 <= x < N).
+ move=> x N; rewrite size_filter count_uniq_mem.
+  by apply range_uniq. 
+ by rewrite mem_range.
+rewrite !L size_filter; clear L.
+rewrite (eq_in_count _ (fun x => x=(x2*2^k1+x1) /\ 0 <= x1 < 2^k1)).
+ move => x /mem_range [Hx1 Hx2] /=.
+ rewrite /pred1 /=; split.
+  move => [<- <-] //.
+  rewrite -divz_eq /=.
+  smt(modz_ge0 ltz_mod expr_gt0).
+ move => [-> [??]]; split.
+  by rewrite addrC modzMDr modz_small /#.
+ by rewrite addrC divzMDr 1:/# divz_small /#.
+rewrite !ler_maxr; first 3 by smt(expr_gt0).
+rewrite -!fromintM -exprD_nneg; first 2 by smt(expr_gt0).
+congr.
+have ->: forall (y:int) b l, uniq l => count (fun x => (x=y) /\ b) l = b2i (y \in l /\ b).
+  move=> y b; case: b => Hb /=.
+   by elim => //= x xs IH [Hxs Hun]; rewrite IH /#.
+  by move=> H Hun; rewrite count_pred0 b2i0.
+ by apply range_uniq.
+case: (0 <= x1 && x1 < 2 ^ k1) => Hx1.
+ rewrite !b2i1 /= mem_range; congr; congr.
+ apply eq_iff; split => H.
+  split; first smt(@IntOrder).
+  move=>_; rewrite exprD_nneg 1..2:/#.
+  have ->: 2 ^ k1 * 2 ^ k2 = 2 ^ k2 * 2 ^ k1 by smt().
+  have ?: x2 * 2 ^ k1 < 2 ^ k2 * 2 ^ k1 by smt(@IntOrder).
+  smt().
+ split; smt(exprD_nneg expr_gt0).
+by rewrite !b2i0.
+qed.
+
+lemma dbitsD k1 k2:
+ 0 <= k1 => 0 <= k2 =>
+ dbits (k1+k2)
+ = dmap (dbits k1 `*` dbits k2) (fun x:int*int=>x.`1 + x.`2 * 2^k1).
+proof.
+move=> Hk1 Hk2.
+rewrite dprod_dbits // dmap_comp /(\o) //=.
+by rewrite dmap_id_eq_in //=; smt(divz_eq).
+qed.
+
+require import BitEncoding DBool DList.
+from Jasmin require JUtils.
+
+import BitEncoding BitChunking BS2Int.
+
+lemma dbits_bs k:
+ 0 <= k =>
+ dbits k = dmap (dlist {0,1} k) bs2int.
+proof.
+elim/natind: k.
+ move=> k ??; have ->: k=0 by smt().
+ rewrite dlist0 1://.
+ rewrite eq_distr; move => x.
+ rewrite dinter1E dmap1E dunitE /(\o) /pred1 /=.
+ by rewrite bs2int_nil /#.
+move=> k Hk IH _.
+rewrite 1!(addrC k) dbitsD //.
+have ->: dbits 1 = dmap (dlist {0,1} 1) bs2int.
+ rewrite dlist1 dmap_comp /(\o) /= eq_distr => x.
+ by rewrite dinter1E dmap1E dboolE /(\o) /pred1 !JUtils.bs2int_cons !bs2int_nil /#.
+rewrite dlist_add // IH //.
+rewrite dmap_dprod !dmap_comp /(\o) /=.
+apply eq_dmap_in => x /=.
+rewrite supp_dprod !supp_dlist //; move=> [[E ?][??]].
+by rewrite JUtils.bs2int_cat E expr1 /#.
+qed.
+
+op spreadbits (k n x: int): int list =
+ mkseq (fun i=> x%/2^(i*k) %% 2^k) n.
+
+lemma spreadbits0 k: spreadbits k 0 = fun n => [].
+proof. by apply fun_ext => x; rewrite /spreadbits mkseq0. qed.
+
+lemma spreadbitsS k n: 
+ 0 <= n =>
+ spreadbits k (n+1) = 
+ fun x => rcons (spreadbits k n x) (x %/ 2 ^ (n * k) %% 2 ^ k).
+proof. 
+move=> Hn.
+by apply fun_ext => x; rewrite /spreadbits mkseqS //; congr.
+qed.
+
+op joinbits (k:int) (l: int list) = foldr (fun x r=>x+2^k*r) 0 l.
+
+lemma spreadbits_modz k n x:
+ 0 <= n => 0 < k => 
+ spreadbits k n x = spreadbits k n (x %% 2^(n*k)).
+proof.
+elim/natind: n k x.
+ move=> n Hn0 k H0n Hk; have ->/=: n=0 by smt().
+ by rewrite !spreadbits0.
+move=> n Hn0 IH k x _ Hk.
+rewrite spreadbitsS //= IH // mulrDl /= eq_sym IH //.
+congr.
+ by congr; apply modz_dvd_pow; smt().
+by rewrite modz_pow2_div 1:/# addrC addrA (addrC _ (n*k)) /= modz_mod.
+qed.
+
+lemma dbits_spreadbits k n:
+ 0 <= n => 0 < k =>
+ dmap (dbits (n*k)) (spreadbits k n)
+ = dlist (dbits k) n.
+proof.
+elim/natind: n k.
+ move=> n Hn0 k H0n; have ->/=: n=0 by smt().
+ move=> H0; rewrite dlist0 // spreadbits0 /=.
+ rewrite eq_distr; move => x. 
+ by rewrite dmap_cst; first by apply dinter_ll.
+move=> n Hn IH k size Hk.
+rewrite dlistSr // mulrDl /=.
+rewrite dbitsD 1..2:/# spreadbitsS //.
+rewrite dmap_comp /(\o) /=.
+rewrite -IH 1..2:/# dmap_dprodL.
+rewrite !dmap_comp /(\o) /=.
+apply eq_dmap_in.
+move=> [x1 x2]; rewrite supp_dprod /= !supp_dinter; move => [H1 H2].
+congr.
+ by rewrite spreadbits_modz // modzMDr modz_small /#.
+rewrite -{2}(modz_small x2 (2^k) _) 1:/#.
+congr; congr.
+by rewrite divzMDr; smt(expr_gt0).
+qed.
+
+module SplitBits = {
+  proc sample_split(k1 k2: int) = {
+    var x, a, b;
+    x <$ dbits (k1+k2);
+    a <- x %% 2^k1;
+    b <- x %/ 2^k1;
+    return (a,b);
+  }
+  proc sample_splitted(k1 k2: int) = {
+    var a, b;
+    a <$ dbits k1;
+    b <$ dbits k2;
+    return (a,b);
+  }
+}.
+
+require import DMap DProd.
+clone DMapSampling as MS with
+ type t1 <- int,
+ type t2 <- int*int.
+clone ProdSampling as PS with
+ type t1 <- int,
+ type t2 <- int.
+
+lemma dbits_split:
+  equiv [ SplitBits.sample_split ~ SplitBits.sample_splitted
+        : ={k1, k2} /\ 0 <= k1{1} /\ 0 <= k2{1} ==> ={res} ].
+proof.
+proc; simplify.
+transitivity {2} { (a,b) <@ PS.S.sample2(dbits k1, dbits k2); }
+ ( ={k1,k2} /\ 0 <= k1{1} /\ 0 <= k2{1} ==> ={a,b} )
+ ( ={k1,k2} /\ 0 <= k1{1} /\ 0 <= k2{1} ==> ={a,b} ).
+- by move=> /> &m *; exists k1{m} k2{m} => /#.
+- smt().
+- transitivity {2} { (a,b) <@ PS.S.sample(dbits k1, dbits k2); }
+   ( ={k1,k2} /\ 0 <= k1{1} /\ 0 <= k2{1} ==> ={a,b} )
+   ( ={k1,k2} /\ 0 <= k1{1} /\ 0 <= k2{1} ==> ={a,b} ).
+  + by move=> /> &m *; exists k1{m} k2{m} => /#.
+  + smt().
+  + inline*.
+    transitivity {2} { (a,b) <@ MS.S.sample(dbits (k1+k2), fun x => (x%%2^k1, x%/2^k1)); }
+     ( ={k1,k2} /\ 0 <= k1{1} /\ 0 <= k2{1} ==> ={a,b} )
+     ( ={k1,k2} /\ 0 <= k1{1} /\ 0 <= k2{1} ==> ={a,b} ).
+    * by move=> /> &m *; exists k1{m} k2{m} => /#.
+    * smt().
+    * transitivity {2} { (a,b) <@ MS.S.map(dbits (k1+k2), fun x => (x%%2^k1, x%/2^k1)); }
+       ( ={k1,k2} /\ 0 <= k1{1} /\ 0 <= k2{1} ==> ={a,b} )
+       ( ={k1,k2} /\ 0 <= k1{1} /\ 0 <= k2{1} ==> ={a,b} ).
+      - by move=> /> &m *; exists k1{m} k2{m} => /#.
+      - smt().
+      - inline*; auto. 
+      - by symmetry; call MS.sample; auto.
+    * inline*; wp; rnd; wp; skip => /> &m Hk1 Hk2.
+      by rewrite dprod_dbits.
+  + by call PS.sample_sample2; auto.
+- by inline*; auto.
+qed.
+
+module JoinBits = {
+  proc sample_join(k1 k2: int) = {
+    var a, b;
+    a <$ dbits k1;
+    b <$ dbits k2;
+    return a + b * 2^k1;
+  }
+  proc sample_joined(k1 k2: int) = {
+    var x;
+    x <$ dbits (k1+k2);
+    return x;
+  }
+}.
+
+lemma dbits_join:
+  equiv [ JoinBits.sample_join ~ JoinBits.sample_joined
+        : ={k1, k2} /\ 0 <= k1{1} /\ 0 <= k2{1} ==> ={res} ].
+proof.
+proc; simplify.
+transitivity {1} { (a,b) <@ SplitBits.sample_split(k1,k2); }
+ ( ={k1, k2} /\ 0 <= k1{1} /\ 0 <= k2{1} ==> ={a,b,k1,k2} )
+ ( ={k1, k2} /\ 0 <= k1{1} /\ 0 <= k2{1} ==> a{1} + b{1} * 2 ^ k1{1} = x{2} ).
+- by move => /> &m ??; exists k1{m} k2{m}.
+- by [].
+- transitivity {2} { (a,b) <@ SplitBits.sample_splitted(k1, k2); }
+   ( ={k1, k2} /\ 0 <= k1{1} /\ 0 <= k2{1} ==> ={a,b,k1,k2} )
+   ( ={k1, k2} /\ 0 <= k1{1} /\ 0 <= k2{1} ==> ={a,b,k1,k2} ).
+  + by move => /> &m ??; exists k1{m} k2{m}.
+  + by [].
+  + by inline*; wp; rnd; rnd; auto.
+  + by symmetry; call dbits_split; auto.
+- inline*; wp; rnd; wp; skip => /> &m Hk1 Hk2 x Hx.
+  smt(divz_eq).
+qed.
+
+require import Binomial.
+
+(* CENTERED BINOMIAL DISTRIBUTION *)
+op mcbd (eta_ x: int) =
+  (bin (2*eta_) (x+eta_))%r * (inv 2%r)^(2*eta_).
+
+op dcbd (eta_: int): int distr =
+ dmap (dbin (inv 2%r) (2*eta_)) (fun x => x-eta_).
+
+lemma dbin1E_half n k:
+ mu1 (dbin (inv 2%r) n) k = (bin n k)%r * (inv 2%r ^ n).
+proof. by rewrite dbin1E; smt(@Real). qed.
+
+lemma dcbd1E eta_ x:
+ mu1 (dcbd eta_) x = mcbd eta_ x.
+proof.
+rewrite dmap1E /(\o) /=.
+rewrite (mu_eq _ _ (pred1 (x+eta_))) 1:/#.
+by rewrite dbin1E_half /#.
+qed.
+
+lemma gt0_bin n k:
+ 0 < bin n k <=> 0 <= k <= n.
+proof.
+split => [H|[]].
+ apply contraT.
+ rewrite andaE negb_and; move=> [?|?].
+  by move: H; rewrite bin_lt0r /#.
+ by move: H; rewrite bin_gt /#.
+elim/natind: k n; first by smt(bin0).
+move=> k Hk0 IH n _ Hkn.
+rewrite (_:n=n-1+1) 1:/# binSn 1..2:/#.
+move: (IH (n-1) _ _); smt(ge0_bin).
+qed.
+
+lemma supp_dcbd eta_ x:
+ x\in (dcbd eta_) <=> -eta_ <= x <= eta_.
+proof.
+rewrite /support dcbd1E /mcbd.
+have ->: (-eta_ <= x && x <= eta_) = (0 < bin (2 * eta_) (x + eta_))
+ by smt(gt0_bin).
+smt(@RealOrder).
+qed.
+
+lemma ll_dcbd eta_:
+ 0 <= eta_ =>
+ is_lossless (dcbd eta_).
+proof. by move=> Heta; apply dmap_ll; apply ll_dbin; smt(). qed.
+
+lemma mcbd_2_2N: mcbd 2 (-2) = inv 16%r.
+proof.
+by rewrite /mcbd /= bin0 // RField.exprVn //= RField.fromintXn //=.
+qed.
+
+lemma bin_4_1: bin 4 1 = 4.
+proof.
+by rewrite (_:4=0+1+1+1+1) // (_:1=0+1) // !binSn // !bin0 // !bin0n !b2i0 /=.
+qed.
+
+lemma mcbd_2_1N: mcbd 2 (-1) = 4%r / 16%r.
+proof.
+by rewrite /mcbd /= bin_4_1 // RField.exprVn //= RField.fromintXn //=.
+qed.
+
+lemma bin_4_2: bin 4 2 = 6.
+proof.
+by rewrite (_:4=0+1+1+1+1) // (_:2=0+1+1) // !binSn // !bin0 // !bin0n !b2i0 /=.
+qed.
+
+lemma mcbd_2_0: mcbd 2 0 = 6%r / 16%r.
+proof.
+by rewrite /mcbd /= bin_4_2 // RField.exprVn //= RField.fromintXn //=.
+qed.
+
+lemma bin_4_3: bin 4 3 = 4.
+proof.
+rewrite (_:4=0+1+1+1+1) // (_:3=0+1+1+1) // !binSn // !bin0 // !bin0n /#.
+qed.
+
+lemma mcbd_2_1: mcbd 2 1 = 4%r / 16%r.
+proof.
+by rewrite /mcbd /= bin_4_3 // RField.exprVn //= RField.fromintXn //=.
+qed.
+
+lemma mcbd_2_2: mcbd 2 2 = inv 16%r.
+proof.
+by rewrite /mcbd /= binn // RField.exprVn //= RField.fromintXn //=.
+qed.
+
+lemma mcbd_3_3N: mcbd 3 (-3) = inv 64%r.
+proof.
+by rewrite /mcbd /= bin0 // RField.exprVn //= RField.fromintXn //=.
+qed.
+
+lemma bin_6_1: bin 6 1 = 6.
+proof.
+by rewrite (_:6=0+1+1+1+1+1+1) // (_:1=0+1) // !binSn // !bin0 // !bin0n !b2i0 /=.
+qed.
+
+lemma mcbd_3_2N: mcbd 3 (-2) = 6%r / 64%r.
+proof.
+by rewrite /mcbd /= bin_6_1 // RField.exprVn //= RField.fromintXn //=.
+qed.
+
+lemma bin_6_2: bin 6 2 = 15.
+proof.
+by rewrite (_:6=0+1+1+1+1+1+1) // (_:2=0+1+1) // !binSn // !bin0 // !bin0n !b2i0 /=. 
+qed.
+
+lemma mcbd_3_1N: mcbd 3 (-1) = 15%r / 64%r.
+proof.
+by rewrite /mcbd /= bin_6_2 // RField.exprVn //= RField.fromintXn //=.
+qed.
+
+lemma bin_6_3: bin 6 3 = 20.
+proof.
+by rewrite (_:6=0+1+1+1+1+1+1) // (_:3=0+1+1+1) // !binSn // !bin0 // !bin0n !b2i0 /=.
+qed.
+
+lemma mcbd_3_0: mcbd 3 0 = 20%r / 64%r.
+proof.
+by rewrite /mcbd /= bin_6_3 // RField.exprVn //= RField.fromintXn //=.
+qed.
+
+lemma bin_6_4: bin 6 4 = 15.
+proof.
+by rewrite (_:6=0+1+1+1+1+1+1) // (_:4=0+1+1+1+1) // !binSn // !bin0 // !bin0n !b2i0 /=. 
+qed.
+
+lemma mcbd_3_1: mcbd 3 1 = 15%r / 64%r.
+proof.
+by rewrite /mcbd /= bin_6_4 // RField.exprVn //= RField.fromintXn //=.
+qed.
+
+lemma bin_6_5: bin 6 5 = 6.
+proof.
+by rewrite (_:6=0+1+1+1+1+1+1) // (_:5=0+1+1+1+1+1) // !binSn // !bin0 // !bin0n !b2i0 /=.
+qed.
+
+lemma mcbd_3_2: mcbd 3 2 = 6%r / 64%r.
+proof.
+by rewrite /mcbd /= bin_6_5 // RField.exprVn //= RField.fromintXn //=.
+qed.
+
+lemma mcbd_3_3: mcbd 3 3 = inv 64%r.
+proof.
+by rewrite /mcbd /= binn // RField.exprVn //= RField.fromintXn //=.
+qed.
+
+(* remove redundant hypothesis from "binSn" *)
+lemma binSn' n m:
+     0 <= n => bin (n + 1) (m + 1) = bin n (m + 1) + bin n m.
+proof.
+case: (0 <= m) => Hm Hn.
+ by rewrite binSn.
+case: (m+1 < 0) => H.
+ by rewrite !bin_lt0r //#.
+have ->: (m+1 = 0) by smt().
+by rewrite !bin0 1..2:/# bin_lt0r /#.
+qed.
+
+lemma aux n k:
+ 0 <= n =>
+ bin (2*(n+1)) (k+(n+1))
+ = 2*bin (2*n) (k+n) + bin (2*n) (k+n-1) + bin (2*n) (k+n+1).
+proof.
+move=> Hn.
+have ->: 2*(n+1) = 2*n + 1 + 1 by ring.
+rewrite addrA binSn' 1:/# binSn' 1:/# addrC.
+by rewrite (_:k+n=k+n-1+1) 1:/# binSn' /#.
+qed.
+
+(*
+from Jasmin require import JWord JWord_array.
+
+import BitEncoding BitChunking BS2Int.
+*)
+
+abbrev hamming_weight l = count (fun x=>x) l.
+
+op dcbd_sample eta_ =
+ dmap (dlist {0,1} eta_ `*` dlist {0,1} eta_)
+      (fun ll:_*_ => hamming_weight ll.`1 - hamming_weight ll.`2).
+
+lemma dcbd_sampleS eta_:
+ 0 <= eta_ =>
+ dcbd_sample (eta_ + 1)
+ = dmap (({0,1}`*`{0,1}) `*` (dlist {0,1} eta_ `*` dlist {0,1} eta_))
+        (fun x:(_*_)*(_*_) => b2i x.`1.`1 - b2i x.`1.`2
+           + hamming_weight x.`2.`1 - hamming_weight x.`2.`2).
+proof.
+move => Hn; rewrite /dcbd_sample dlistS // /dapply /=.
+rewrite dmap_dprod dmap_comp /(\o) /=.
+pose d1:= _ `*` _ `*` (_ `*` _).
+pose d2:= {0,1} `*` {0,1} `*` _.
+have ->:
+ d1 = dmap d2 (fun x:(_*_)*(_*_) => 
+               ((x.`1.`1,x.`2.`1),(x.`1.`2,x.`2.`2))).
+ rewrite eq_distr; move => [[k11 k12][k21 k22]].
+ rewrite !dmap1E.
+ pose f := _\o _; have ->: f = pred1 ((k11,k21),(k12,k22)).
+  by rewrite /f /pred1 fun_ext; move => [[??][??]] /#.
+ by rewrite !dprod1E /#. 
+rewrite dmap_comp /(\o).
+apply eq_dmap_in; move => [[h1 h2][t1 t2]].
+by rewrite !supp_dprod /=; move => [[??][??]] /#.
+qed.
+
+lemma dcbd_eq_sample eta_:
+ 0 <= eta_ =>
+ dcbd eta_ = dcbd_sample eta_.
+proof.
+move=> Heta; rewrite eq_distr; move => k.
+elim/natind: eta_ Heta k.
+ move=> n ?? k; rewrite (_:n=0) 1:/# dcbd1E /mcbd RField.expr0 /=.
+ rewrite /dcbd_sample dlist0 // dmap1E /(\o) /pred1 bin0n /=.
+ case: (k=0) => [->|E].
+  rewrite (mu_eq_support _ _ (fun x:_*_=>x.`1=[] /\ x.`2=[])).
+   by move=> [l1 l2]; rewrite supp_dprod !supp_dunit /#.
+  by rewrite (dprodE (pred1 []) (pred1 [])); smt(dunit1E).
+ rewrite (mu_eq_support _ _ pred0).
+  by move=> [l1 l2]; rewrite supp_dprod !supp_dunit /#.
+ by rewrite mu0.
+move=> n Hn IH _ k.
+rewrite dcbd_sampleS // dmap_dprodE /=.
+rewrite (dlet1Efin _ _ _ [(false,false);(false,true);(true,false);(true,true)]).
+ move => [] /= x1 x2.
+ by rewrite supp_dprod !supp_dbool /#.
+rewrite /= !big_consT big_nil /=.
+pose f (y:_*_) := hamming_weight y.`1 - hamming_weight y.`2.
+pose fp (y:_*_) := 1 + hamming_weight y.`1 - hamming_weight y.`2.
+pose fm (y:_*_) := -1 + hamming_weight y.`1 - hamming_weight y.`2.
+rewrite (eq_dmap _ fm ((fun x=> -1 + x)\o f)) 1:/#.
+rewrite (eq_dmap _ fp ((fun x=> 1 + x)\o f)) 1:/#.
+rewrite -2!dmap_comp -/(dcbd_sample n).
+rewrite (dmap1E_can _ (fun x=>(-1)+x) (fun x=>x+1)) //.
+rewrite (dmap1E_can _ (fun x=>1+x) (fun x=>x-1)) //.
+rewrite -!IH // !dprod1E !dbool1E /= !dcbd1E /mcbd.
+rewrite aux // mulzDr /=.
+have ->: inv 2%r ^ (2 * n + 2) = inv 2%r ^ (2 * n) / (2^2)%r.
+ rewrite RField.exprD 1:/#; field; smt().
+smt().
+qed.
+
+
+
+module RejSampling = {
+ proc sample_upto(max: int) = {
+  var x;
+  x <$ [0..max];
+  return x;
+ }
+ proc samplelist_upto(max n: int) = {
+  var l;
+  l <$ dlist [0..max] n;
+  return l;
+ }
+ proc rsample(k max: int) = {
+  var x;
+  x <$ dbits k;
+  while (max < x) {
+   x <$ dbits k;  
+  }
+  return x;
+ }
+ proc rmodsample(k rmax max: int) = {
+  var x;
+  x <$ dbits k;
+  while (rmax < x) {
+   x <$ dbits k;  
+  }
+  return x %% (max+1);
+ }
+(*
+ proc rsamplelist(k max n: int) = {
+  var x, j, y: int;
+  var l;
+  j <- 0;
+  l <- [];
+  while (j < n) {
+   x <$ dbits k;
+   if (x <= max) {
+    l <- rcons l x;
+    j <- j+1;
+   }
+  }
+  return l;
+ }
+*)
+ proc rsamplelist(k max n: int) = {
+  var x, i, j, y: int;
+  var l;
+  i <- 0;
+  j <- 0;
+  l <- [];
+  while (j < n) {
+   x <$ dbits k;
+   if (x <= max) {
+    l <- rcons l x;
+    j <- j+1;
+   }
+   i <- i+1;
+  }
+  return l;
+ }
+(*
+ proc rsamplelist3(k max n nchunk: int) = {
+  var x, i, j, y: int;
+  var xl, l;
+  i <- 0;
+  j <- 0;
+  xl <- [];
+  l <- [];
+  while (j < n) {
+   if (xl = []) xl <- nseq nchunk (dbits k);
+   x <$ head (dunit 0) xl;
+   xl <- behead xl;
+   if (x <= max) {
+    l <- rcons l x;
+    j <- j+1;
+   }
+   i <- i+1;
+  }
+  return l;
+ }
+*)
+ proc rsamplelist_chunked(k max n nchunk: int) = {
+  var i, j, xn, x: int;
+  var xx, xl, l: int list;
+  var dxx: int distr;
+  i <- 0;
+  j <- 0;
+  l <- [];
+  while (j < n) {
+   xn <- 0;
+   while (xn < nchunk && j < n) {
+    x <$ dbits k;
+    if (x <= max ) {
+     l <- rcons l x;
+     j <- j + 1;
+    }
+    xn <- xn+1;
+   }
+   i <- i+1;
+  }
+  return l;
+ }
+(*
+ proc rsamplelist_chunked(k max n nchunk: int) = {
+  var i, j, xn, x: int;
+  var xx, xl, l: int list;
+  var dxx: int distr;
+  i <- 0;
+  j <- 0;
+  l <- [];
+  while (j < n) {
+   xl <$ dlist (dbits k) nchunk;
+   xn <- 0;
+   while (xn < nchunk && j < n) {
+    x <- nth 0 xl xn;
+    if (x <= max ) {
+     l <- rcons l x;
+     j <- j + 1;
+    }
+    xn <- xn+1;
+   }
+   i <- i+1;
+  }
+  return l;
+ }
+ proc rsamplelist_chunked3(k max n nchunk: int) = {
+  var i, j: int;
+  var xx, xl, l: int list;
+  var dxx: int distr;
+  i <- 0;
+  j <- 0;
+  l <- [];
+  while (j < n) {
+   xx <$ dlist (dbits k) nchunk;
+   (*dxx <- nseq nchunk (dbits k);
+   xx <$ djoin dxx;*)
+   xl <- take (n-j) (filter (fun x=> x<=max) xx);
+   j <- j + size xl;
+   i <- i+1;
+  }
+  return l;
+ }
+*)
+}.
+
+equiv rsample_chunked_eq:
+ RejSampling.rsamplelist ~  RejSampling.rsamplelist_chunked
+ : ={k,max,n} /\ 0 < nchunk{2} ==> ={res}.
+proc; simplify.
+exlim nchunk{2} => _N.
+async while
+ [ (fun x => i < _N*x), i{2}+1 ]
+ [ (fun x => i < x), i{2}+1 ]
+ ( j{1}<n{1} /\ j{2}<n{2}) ( ! j{2}<n{2} )
+ : (={k,max,n,j,l} /\ (n{1}<=j{1} \/ i{1}=_N*i{2}) /\ 0<=i{1} /\ _N=nchunk{2} /\ 0 < _N).
++ by move=> /> &2 /#.
++ by move=> /> &2 /#.
++ by move=> /> &2 *. 
++ by move=> &2; wp; rnd; auto.
++ move=> /> &1; exfalso; smt().
++ move=> v1 v2.
+  rcondt{2} 1; 1: by auto => /> /#.
+  rcondf{2} 4.
+   by move=> &m; wp; while true; auto.
+  exlim i{1} => i0.
+  wp; while (={k,max,n,k,j,l} /\ _N = nchunk{2} /\ 0<_N /\ (n{2}<=j{2} \/ i{1}=i{2}*_N+xn{2}) /\ xn{2}<=_N /\ 0<=i{1} /\ v1=i{2}+1 /\ v2=i{2}+1).
+   by wp; auto => /> &1 &2 /#. 
+  by wp; auto => /> /#. 
++ by rcondf 1; auto; smt().
++ by rcondf 1; auto; smt().
+by wp; auto.
+qed.
+
+require import Dexcepted.
+
+clone WhileSampling as WS with
+ type input <- int*int,
+ type t <- int,
+ op dt (i:int*int) = dbits i.`2.
+
+equiv rsample_upto: 
+ RejSampling.sample_upto ~ RejSampling.rsample: 
+ ={max} /\ 0 <= max{2} < 2^k{2} ==> ={res}.
+proof.
+transitivity WS.SampleE.sample
+ (0 <= max{1} < 2^i{2}.`2 /\ max{1}=i{2}.`1 /\ test{2} =(fun (i:int*int) x => i.`1 < x) ==> ={res})
+ (i{1}.`1=max{2} /\ i{1}.`2=k{2} /\ test{1} =(fun (i:int*int) x => i.`1 < x ) ==> ={res}).
+- move=> /> &m ??; exists ((max{m},k{m}),fun (i:_*_) x=>i.`1 < x)%Int; smt().
+- done.
+- proc; rnd; auto => /> &m ??; split.
+   move=> x Hx.
+   have HH: 0 <= x <= i{m}.`1.
+    by move: Hx; rewrite supp_dexcepted supp_dinter /#.
+   rewrite dexcepted1E.   
+   rewrite (_:i{m}.`1 < x = false) 1:/#/=.
+   rewrite !dinter1E.
+   rewrite (_:0 <= x && x <= 2 ^ i{m}.`2 - 1) 1:/#/=.
+   rewrite (_:0 <= x && x <= i{m}.`1) 1:/#/=.
+   rewrite weight_dinter.
+   rewrite (_:0 <= 2 ^ i{m}.`2 - 1).
+    smt(StdOrder.IntOrder.expr_gt0).
+   rewrite dinterE /= StdOrder.IntOrder.ler_maxr /=.
+    smt(StdOrder.IntOrder.expr_gt0).
+   rewrite (range_cat (i{m}.`1+1)) 1..2:/#.
+   rewrite filter_cat eq_in_filter_pred0 /=.
+    smt(mem_range).
+   rewrite eq_in_filter_predT.
+    smt(mem_range).
+   rewrite size_range StdOrder.IntOrder.ler_maxr /#.
+  move=> H x Hx.
+  have HH: 0 <= x <= i{m}.`1.
+   by move: Hx; rewrite supp_dinter /#.
+  by rewrite supp_dexcepted supp_dinter /#.
+- transitivity WS.SampleW.sample
+   (={i,test} ==> ={res})
+   (i{1}.`1=max{2} /\ i{1}.`2=k{2} /\ test{1} =(fun (m:_*_) x => m.`1 < x)%Int ==> ={res}).
+  + by move=> /> &1 &2 *; exists (i{1},(fun (i:_*_) x => i.`1 < x)%Int); smt().
+  + done.
+  + conseq WS.sampleE_sampleW.
+    move=> /> &1 &2 *; rewrite dinter_ll.
+    smt(StdOrder.IntOrder.expr_gt0).
+- proc; inline*; simplify.
+  wp; while (test0{1}=(fun (i:_*_) x=>i.`1<x)%Int /\ r0{1}=x{2}/\i0{1}=(max{2},k{2})).
+   by rnd; skip => /> &1 &2 *.
+  by wp; rnd; skip => /> &m * /#.
+qed.
+
+clone DMapSampling as MS2 with
+ type t1 <- int,
+ type t2 <- int.
+
+equiv rmodsample_upto: 
+ RejSampling.sample_upto ~ RejSampling.rmodsample: 
+ ={max} /\ 0 <= max{2} /\ 0 <= rmax{2} < 2^k{2} /\ (max{2}+1)%|(rmax{2}+1) ==> ={res}.
+proof.
+proc; simplify.
+transitivity {2} { x <@ RejSampling.rsample(k, rmax); }
+ ( ={max} /\ 0<=max{2} /\ 0 <= rmax{2} && rmax{2} < 2 ^ k{2} /\ (max{2}+1) %| (rmax{2}+1) ==> x{1}=x{2}%%(max{2}+1) )
+ ( ={max} /\ ={k,rmax} /\ (0 <= rmax{2} && rmax{2} < 2 ^ k{2}) /\ (max{2}+1) %| (rmax{2}+1) ==> ={x,max} ).
+- by move=> /> &m *; exists k{m} max{m} rmax{m}.
+- done.
+- transitivity {2} { x <@ RejSampling.sample_upto(rmax); }
+   ( ={max} /\ 0<=max{2} /\ 0 <= rmax{2} && rmax{2} < 2 ^ k{2} /\ (max{2}+1) %| (rmax{2}+1) ==> x{1}=x{2}%%(max{2}+1) )
+   ( ={max,rmax,k} /\ (0 <= rmax{2} && rmax{2} < 2 ^ k{2}) /\ (max{2}+1) %| (rmax{2}+1) ==> ={x,max} ).
+  + by move=> /> &m *; exists k{m} max{m} rmax{m}.
+  + done.
+  + transitivity {2} { x <@ MS2.S.sample([0..rmax],fun x=>x%%(max+1)); }
+     ( ={max} /\ 0<=max{2} /\ 0<=rmax{2} /\ (max{2}+1) %| (rmax{2}+1) ==> ={x} )
+     ( ={max,rmax} /\ (0 <= rmax{2} && rmax{2} < 2 ^ k{2}) /\ (max{2}+1) %| (rmax{2}+1) ==> x{1}=x{2}%%(max{2}+1) ).
+    * by move=> /> &m *; exists max{m} rmax{m}.
+    * done.
+    * inline*; wp; rnd; auto => /> &m *.
+      by rewrite -(duni_range_dvd (rmax{m}+1) (max{m}+1)) /#.
+    transitivity {1} { x <@ MS2.S.map([0..rmax], fun x=>x%%(max+1)); }
+     (={max,rmax} ==> ={x})
+     (={max,rmax} ==> ={rmax} /\ x{1} = x{2} %% (max{2} + 1)).
+    * by move=> /> &m *; exists max{m} rmax{m}.
+    * done.
+    * by call MS2.sample; auto.
+    by inline*; wp; rnd; auto.
+  by call rsample_upto.
+- by inline*; sim.
+qed.
+
+abstract theory ProgramDList.
+  type t.
+
+  module Sample = {
+    proc sample(d: t distr, n:int): t list = {
+      var r;
+
+      r <$ dlist d n;
+      return r;
+    }
+  }.
+
+  module SampleCons = {
+    proc sample(d: t distr, n:int): t list = {
+      var r, rs;
+
+      rs <$ dlist d (n - 1);
+      r  <$ d;
+      return r::rs;
+    }
+  }.
+
+lemma pr_Sample (_d: t distr) _n &m xs:
+ Pr[Sample.sample(_d,_n) @ &m: res = xs]
+ = mu (dlist _d _n) (pred1 xs).
+  proof. by byphoare (_: d = _d /\ n = _n ==> res = xs)=> //=; proc; rnd. qed.
+
+equiv Sample_SampleCons_eq:
+ Sample.sample ~ SampleCons.sample: 
+  0 < n{1} /\ ={d,n} ==> ={res}.
+proof.
+bypr (res{1}) (res{2})=> //= &1 &2 xs [lt0_n] [<- <-].
+rewrite (pr_Sample d{1} n{1} &1 xs); case (size xs = n{1})=> [En|].
+case xs En lt0_n=> [|x xs E lt0_n]; 1:smt().
+ rewrite -E dlistS1E.
+ byphoare (_: d=d{1} /\ n = size xs + 1 ==> x::xs = res)=> //=; last by smt().
+ proc; simplify.
+ seq 1: (rs = xs) (mu (dlist d{1} (size xs)) (pred1 xs)) (mu d (pred1 x)) _ 0%r.
+ + done.
+ + by rnd (pred1 xs); skip; smt().
+ + by rnd (pred1 x); skip; smt().
+ + by hoare; auto; smt().
+ + smt().
+move=> len_xs; rewrite dlist1E 1:/# (_: n{1} <> size xs) /= 1:/#.
+byphoare (_: n = n{1} ==> xs = res)=> //=; hoare.
+by proc; auto => /> &m l; rewrite supp_dlist /#.
+qed.
+
+end ProgramDList.
+
+clone ProgramDList as P with type t <- int.
+
+equiv rsamplelist_upto: 
+ RejSampling.samplelist_upto ~ RejSampling.rsamplelist: 
+ ={max,n} /\ 0 <= max{2} < 2^k{2} ==> ={res}.
+proof.
+proc; simplify.
+exlim n{1} => N; elim/natind: N => [|N HN IH].
+ move=> n H0.
+ rnd {1}.
+ rcondf {2} 4.
+  by move=> &m; wp; skip; smt().
+ wp; skip => /> &m *.
+ by rewrite !dlist0 //; smt(dunit_ll supp_dunit).
+transitivity {1} { l <@ P.SampleCons.sample([0..max],n); }
+ ( 0 < n{1} /\ ={max,n} /\ 0 <= max{2} ==> ={l} )
+ ( N+1 = n{1} /\ ={max,n} /\ 0 <= max{2} && max{2} < 2 ^ k{2} ==> ={l} ).
+- by move=> /> &m *; exists max{m} (N+1); auto; smt().
+- done.
+- transitivity {1} { l <@ P.Sample.sample([0..max], n); }
+   ( 0 < n{1} /\ ={max,n} /\ 0 <= max{2} ==> ={l} )
+   ( 0 < n{1} /\ ={max,n} /\ 0 <= max{2} ==> ={l} ).
+  + by move=> /> &m *; exists max{m} n{m}; auto.
+  + done.
+  + by inline*; wp; rnd; wp; auto.
+  + by call P.Sample_SampleCons_eq; skip; smt().
+  inline*.
+  swap {1} 4 -1.
+  transitivity {1}
+   { r <$ [0..max];
+     l <$ dlist [0..max] n;
+     l <- r::l;
+   }
+   (N+1 = n{1} /\ N=n{2} /\ ={max} ==> ={l})
+   (N = n{1} /\ N+1=n{2} /\ ={max} /\ 0 <= max{2} && max{2} < 2 ^ k{2} ==> ={l}).
+  + by move=> /> &1 ??; exists max{1} (N); smt().
+  + done.
+  + by inline*; wp; rnd; wp; rnd; auto.
+  transitivity {2}
+   { i <- 0;
+     j <- 0;
+     while ( j<1 ) {
+       y <$ dbits k;
+       if (y <= max) {
+         j <- j+1;
+       }
+       i <- i+1;
+     }
+     i <- 0;
+     j <- 0;
+     l <- [];
+     while (j < n) {
+       x <$ dbits k;
+       if (x <= max) {
+         l <- rcons l x;
+         j <- j+1;
+       }
+       i <- i+1;
+     }
+     l <- y::l;
+  }
+  ( N=n{1} /\ ={max,n} /\ 0 <= max{2} && max{2} < 2 ^ k{2} ==> ={l})
+  ( N=n{1} /\ N+1=n{2} /\ ={max,k} /\ 0 <= max{2} && max{2} < 2 ^ k{2} ==> ={l}).
+  + by move=> /> &m *; exists k{m} max{m} N; auto.
+  + done.
+  + seq 1 3: (#pre /\ r{1}=y{2}).
+     clear IH.
+     transitivity {1} { r <@ RejSampling.sample_upto(max); }
+      ( N = n{1} /\ ={max, n} 
+       ==> N = n{1} /\ ={r,max,n}  )
+      ( N = n{1} /\ ={max, n} /\ 0 <= max{2} && max{2} < 2 ^ k{2}
+       ==> N = n{1} /\ r{1}=y{2} /\ ={max,n} /\ 0 <= max{2} && max{2} < 2 ^ k{2} ).
+     * by move=> /> &m *; exists max{m} N.
+     * done.
+     * by inline*; wp; rnd; auto.
+     transitivity {2} { y <@ RejSampling.rsample(k,max); }
+      ( N = n{1} /\ ={max, n} /\ 0 <= max{2} && max{2} < 2 ^ k{2}
+       ==> N = n{1} /\ r{1}=y{2} /\ ={max,n}  )
+      ( N = n{1} /\ ={max,k,n} /\ 0 <= max{2} && max{2} < 2 ^ k{2}
+       ==> N = n{1} /\ ={y,max,n} /\ 0 <= max{2} && max{2} < 2 ^ k{2} ).
+     * by move=> /> &m *; exists k{m} max{m} N.
+     * done.
+     * by call rsample_upto. 
+     inline*; wp.
+     unroll {2} 3; rcondt {2} 3; first by auto.
+     seq 3 4: (#pre /\ (k0,max0,x0){1}=(k,max,y){2} /\ (j=b2i (y<=max)){2}).
+      by wp; rnd; auto.
+     while (#pre).
+      by wp; rnd; auto; smt(). 
+     wp; skip; smt().
+    inline*; wp; simplify.
+    by conseq IH.
+  + splitwhile {2} 4 : (j < 1).
+    wp.
+    while (j{1}+1=j{2} /\ #pre /\ y{1}::l{1} = l{2}).
+     wp; rnd; skip => /> &1 &2 *; smt().
+    wp; while (={j,k,max} /\ 0<=j{1}<=1 /\ (0<j{1} => l{2}=[y{1}]) /\ (0=j{1} => l{2}=[])).
+     by wp; rnd; skip => /> &m * /#.
+    by wp; skip => /> &1 &2 * /#.
+qed.
+
+(*
+
+
+
+module ParseShake128 = {
+ (* shake128: blocksize=1600-2*128=1344bit=168byte
+    168 / 3 = 56 *)
+ proc parse_real() = {
+  var j, i: int;
+  var x, xl, l;
+  l <- [];
+  j <- 0;
+  while (j < 256) {
+(* chunk <$ dbits (1344);
+   x <- spreadbits 12 112 chunk; *)
+   i <- 0;
+   xl <- [];
+   while (i < 112) {
+    x <$ dbits 12;
+    xl <- rcons xl x;
+    x <$ dbits 12;
+    xl <- rcons xl x;
+    i <- i + 2;
+   }
+   i <- 0;
+   while (i < 112) {
+    if (nth 0 xl i <= 3329 && j < 256) {
+     l <- rcons l (nth 0 xl i);
+     j <- j + 1;
+    }
+    if (nth 0 xl (i+1) <= 3329 && j < 256) {
+     l <- rcons l (nth 0 xl (i+1));
+     j <- j + 1;
+    }
+    i <- i + 2;
+   }
+  }
+  return l;
+ }
+ proc parse_ideal() = {
+  var l;
+  l <$ dlist [0..3328] 256;
+  return l;
+ }
+}.
+
+equiv parse_dlist:
+ RejSampling.samplelist_upto ~ ParseShake128.parse_real :
+ max{1}=3328 /\ n{1}=256 ==> ={res}.
+proof.
+transitivity RejSampling.rsamplelist
+ (max{1}=3328 /\ n{1}=256 /\ ={max,n} /\ k{2}=12 ==> ={res})
+ (max{1}=3328 /\ n{1}=256 /\ k{1}=12 ==> ={res}).
+- by move=> /> &m *; exists (12,max{m},n{m}).
+- done.
+- conseq rsamplelist_upto => /> *. admit.
+- proc; simplify.
+(*  fusion{2} 3.2@ 1, 2.*)
+  admit.
+
+(* possivel solução:
+rsample por chunks...
+
+split_bits (k:int) (n:int) (x:int): int list
+"split x in a n-list of k-bit integers"
+
+x <$ dbits (k*n)
+l <- split_bits k n x
+==
+l <$ dlist (dbits k) n
+===
+while... (passível de fusion...)
+
+
+
+
+l <- []
+while (0 < n)
+ lchunk <$ dlist (dbits k) nchunk
+ j <- 0
+ l' <- filter R lchunk
+ l <- l ++ take n l'
+ n <- n - size l'
+
+deve dar jeito ter a caracterização de
+dbits vs. dlist dbits n 
+*)
+qed.
+
+op C1: int -> bool.
+op c1:int.
+op C2: int -> bool.
+op c2:int.
+op PRE: bool.
+op SYNC: bool.
+op LR: bool.
+
+equiv xxx: TT.t1 ~ TT.t2 : ={n} ==> ={res}.
+proc.
+conseq (: _ ==> ={l,j}); first by [].
+
+exlim n{1} => N.
+elim/natind: N.
+ admit.
+move => n Hn IH.
+proc.
+
+exlim n{1} => N.
+
+splitwhile {1} 4 : (50 < x).
+unroll {2} 3.
+
+async while
+ [ C1, c1 ]
+ [ C2, c2 ]
+ (={j})
+ (j{1}<j{2})
+ : (={j} => ={l}).
+- move=> &1 &2 Hl. admit (* INSYNC??
+cond{1} \/ cond{2} => SYNC => cond{1} /\ cond{2} /\ C1 c1 /\ C2 c2
+*).
+- move=> &1 &2 Hl. admit (* 
+cond{1} \/ cond{2} => !SYNC => LR => cond{1}
+*).
+- move=> &1 &2 Hl. admit (*
+cond{1} \/ cond{2} => !SYNC => !LR => cond{2}
+*).
+- move=> &m. admit (*
+Context : TT.t1
+
+pre = l = l{m} /\ j < n /\ !SYNC /\ LR
+
+(1--)  x <$ [0..100]            
+(2--)  if (x <= 50) {           
+(2.1)    l <- rcons l x         
+(2.2)    j <- j + 1             
+(2--)  }                        
+
+post = l = l{m}
+*).
+- move=> &m. admit (*
+Context : TT.t2
+
+pre = l{m} = l /\ j < n /\ !SYNC /\ !LR
+
+(1--)  x <$ [0..100]            
+(2--)  while (50 < x) {         
+(2.1)    x <$ [0..100]          
+(2--)  }                        
+(3--)  l <- rcons l x           
+(4--)  j <- j + 1               
+
+post = l{m} = l
+*).
+- move=> v1 v2. admit (*
+&1 (left ) : TT.t1
+&2 (right) : TT.t2
+
+pre = ={l} /\ (cond{1} \/ cond{2}) /\ SYNC /\ v1 = c1 /\ v2 = c2
+
+while (j < n /\ C1 v1) {   (1----)  while (j < n /\ C2 v2) { 
+  x <$ [0..100]            (1.1--)    x <$ [0..100]          
+  if (x <= 50) {           (1.2--)    while (50 < x) {       
+    l <- rcons l x         (1.2.1)      x <$ [0..100]        
+    j <- j + 1             (1.2.2)                           
+  }                        (1.2--)    }                      
+                           (1.3--)    l <- rcons l x         
+                           (1.4--)    j <- j + 1             
+}                          (1----)  }                        
+
+post = ={l}
+*).
+- admit (* LOSSLESS
+Context : TT.t1
+Bound   : [=] 1%r
+
+pre = l = l{2}
+
+(1----)  while (j < n /\ !Inv1 /\ Inv2) {
+(1.1--)    x <$ [0..100]                 
+(1.2--)    if (x <= 50) {                
+(1.2.1)      l <- rcons l x              
+(1.2.2)      j <- j + 1                  
+(1.2--)    }                             
+(1----)  }                               
+
+post = true
+*).
+- admit (* LOSSLESS
+Context : TT.t2
+Bound   : [=] 1%r
+
+pre = l{1} = l
+
+(1----)  while (j_1 < n_1 /\ !Inv1 /\ !Inv2) {
+(1.1--)    x <$ [0..100]                      
+(1.2--)    while (50 < x) {                   
+(1.2.1)      x <$ [0..100]                    
+(1.2--)    }                                  
+(1.3--)    l <- rcons l x                     
+(1.4--)    j <- j + 1                         
+(1----)  }                                    
+
+post = true
+*).
+- by auto.
+qed.
+
+async while
+  [ (fun r => r = (to_uint inlen0)%r), 
+    (to_uint inlen0{2})%r ]
+  [ (fun r => r = (to_uint inlen0)%r), 
+    (to_uint inlen0{1})%r ]
+    (to_uint inlen0{1} = to_uint inlen0{2}) 
+    (to_uint inlen0{2} <= to_uint inlen0{1})
+  :
+    (#{/~ ={in_0}}
+      {~(in_00{2} = in_0{2})}
+      {~(inlen0{1} = inlen{1})}
+      {~(inlen0{2} = inlen{2})}
+      {~(in_0{1} = in_00{2})}
+      {~={r}}
+      {~={h}}pre /\
+      (to_uint inlen{2} - to_uint inlen0{2}) %% 64 = 0 /\
+      (   (* in sync *)
+          (to_uint inlen0{1} = to_uint inlen0{2} /\
+           ={h,r} /\ in_0{1} = in_00{2}) \/
+          (* 3 ahead *)
+          (to_uint inlen0{1} - 3*16 = to_uint inlen0{2} /\
+           ={r} /\ 
+           ((((h{1} + load_block Glob.mem{1} in_0{1}) * r{1}
+              + load_block Glob.mem{1} (in_0{1} + W64.of_int 16)) * r{1})
+                + load_block Glob.mem{1} (in_0{1} + W64.of_int 32)) * r{1}
+                  = h{2} /\
+           in_0{1} + W64.of_int (3*16) = in_00{2}) \/
+          (* 2 ahead *)
+          (to_uint inlen0{1} - 2*16 = to_uint inlen0{2} /\
+           ={r} /\ 
+           (((h{1} + load_block Glob.mem{1} in_0{1}) * r{1}
+              + load_block Glob.mem{1} (in_0{1} + W64.of_int 16)) * r{1}
+                 = h{2})  /\
+           in_0{1} + W64.of_int (2*16) = in_00{2})  \/
+          (* 1 ahead *)
+          (to_uint inlen0{1} - 16 = to_uint inlen0{2} /\
+           ={r} /\ 
+           ((h{1} + load_block Glob.mem{1} in_0{1}) * r{1}
+               = h{2})  /\
+           in_0{1} + W64.of_int 16 = in_00{2})
+      )).
+ (* inv3 => c1 \/ c2 => inv1 => c1 /\ c2 /\ f p /\ g q *)
+ + by rewrite !ultE !uleE /#. 
+ (* inv3 => c1 \/ c2 => !inv1 => inv2 => c1 *)
+ + by rewrite !ultE !uleE /#. 
+ (* inv3 => c1 \/ c2 => !inv1 => !inv2 => c2 *)
+ + by rewrite !ultE !uleE /#. 
+ (* {inv3 /\ c1 /\ !inv1 /\ inv2} Body1 {inv3} *)
+ + move => *; wp; skip; rewrite !ultE !uleE => /> *.
+   by rewrite to_uintB ?uleE //= /#.
+ (* { inv3 /\ c2 /\ !inv1 /\ !inv2} Body2 {inv3} *)
+ + move => *; exfalso; smt().
+ + move => *. 
+   while 
+     (#{/~inlen0{2}}
+              {~in_00{2}}
+              {~={in_0}}
+              {~={r}}
+              {~={h}}
+              {~v1_}
+              {~v2_}pre /\
+       (to_uint inlen{2} - to_uint inlen0{2}) %% 64 = 0 /\ 
+       (  (* in sync *)
+          (to_uint inlen0{1} = to_uint inlen0{2} /\
+           ={h,r} /\ in_0{1} = in_00{2} /\
+          v1_ = (to_uint inlen0{2})%r /\ v2_ = (to_uint inlen0{1})%r) \/
+          (* 3 ahead *)
+          (to_uint inlen0{1} - 3*16 = to_uint inlen0{2} /\
+           ={r} /\ 
+           ((((h{1} + load_block Glob.mem{1} in_0{1}) * r{1}
+              + load_block Glob.mem{1} (in_0{1} + W64.of_int 16)) * r{1})
+                + load_block Glob.mem{1} (in_0{1} + W64.of_int 32)) * r{1}
+                  = h{2} /\
+           in_0{1} + W64.of_int (3*16) = in_00{2} /\
+          v1_ = (to_uint inlen0{2})%r + 64%r /\ v2_ = (to_uint inlen0{1})%r + 16%r) 
+        )).
+    inline *; wp; skip; rewrite !ultE !uleE => /> ????; elim; progress;
+    [ 1,2,8,9: by rewrite ?uleE !to_uintB ?uleE /#
+    | 3,4,10,11: by move: H7 H9; rewrite ?uleE !to_uintB ?uleE /#
+    | 5..7,12..: by move: H7 H8; rewrite ?uleE !to_uintB ?uleE /#
+    ].
+    - skip; rewrite !ultE !uleE => /> ????; elim; progress; smt().
+ (* inv3 ==> islossless while(c1 /\ !inv1 /\ inv2) Body1 *)
+ + while true (W64.to_uint inlen0).
+    by move => *; wp; skip; progress => //=; rewrite to_uintB /#. 
+   by skip; progress; rewrite uleE /#.
+ (* inv3 ==> islossless while(c1 /\ !inv1 /\ !inv2) Body2 *)
+ + while (#pre) (W64.to_uint inlen0).
+    by move => *; wp; skip; rewrite !ultE !uleE => ? /> ??; elim; smt().
+   by skip; rewrite !ultE !uleE => ? /> ??; elim; smt().
+ (* !c1 => !c2 => inv3 => #post *)
+ + skip; rewrite !ultE => /> ????????.
+   rewrite !uleE of_uintK /= negb_and; move => [?|?] /> ??; elim; smt(@W64).
+qed.
+
+
+
+*)
